src/PushButtonSynthesis/SmallExamples.v
@@ -71,7 +71,7 @@ Time Redirect "log" Compute
 Local Existing Instance ToString.C.OutputCAPI.
 Local Existing Instance default_language_naming_conventions.
 Local Existing Instance default_documentation_options.
-Local Instance skip_typedefs : skip_typedefs_opt := true.
+Local Existing Instance default_output_options.
 Local Instance : package_name_opt := None.
 Local Instance : class_name_opt := None.
 Local Instance : static_opt := true.
